byteback-test/test-java-8/src/main/java/byteback/test/generics/Sequences.java
@@ -47,5 +47,6 @@ public abstract class Sequences {
 }
 
 /**
- * RUN: %{verify} %t.bpl
+ * RUN: %{verify} %t.bpl | filecheck %s
+ * CHECK: Boogie program verifier finished with 5 verified, 0 errors
  */
